SystemFD/Metatheory/Preservation.lean
@@ -21,7 +21,7 @@ replace j2 := Term.neutral_form_law (Eq.symm j2); subst j2
 simp at j3; replace j3 := Frame.is_openm_destruct j3
 cases j3; case _ T j3 =>
   have lem := ctx_get_instance_well_typed (judgment_ctx_wf j1) j3 j4
-  apply apply_spine_uniform lem.1 lem.2 j1
+  apply apply_spine_uniform x [] (by simp) lem.1 lem.2 j1
 
 theorem preservation_letterm_lemma :
   Γ ⊢ a : A ->
@@ -32,9 +32,10 @@ theorem preservation_letterm_lemma :
 intro j1 j2 j3
 replace j2 := Term.neutral_form_law (Eq.symm j2); subst j2
 replace j3 := ctx_get_term_well_typed (judgment_ctx_wf j1) (Eq.symm j3)
-apply apply_spine_uniform j3.1 j3.2 j1
+apply apply_spine_uniform x [] (by simp) j3.1 j3.2 j1
 
 theorem preservation_prefix_match_lemma :
+  a.neutral_form = some (x, sp) ->
   Γ ⊢ a : A ->
   Γ ⊢ a.apply_spine ξ : R ->
   Γ ⊢ t : B ->
@@ -42,13 +43,13 @@ theorem preservation_prefix_match_lemma :
   PrefixTypeMatch Γ A B T ->
   Γ ⊢ t.apply_spine ξ : T
 := by
-intro j1 j2 j3 j4 j5
-induction ξ generalizing Γ A R B T a t <;> simp at *
-case _ => sorry
-  -- have lem := uniqueness_of_types j1 j2; subst lem
-  -- replace j4 := stable_type_match_refl_inversion j4
-  -- have lem := prefix_type_match_forced_refl j4 j5; subst lem
-  -- apply j3
+intro js j1 j2 j3 j4 j5
+induction ξ generalizing Γ A R B T a t x sp <;> simp at *
+case _ =>
+  have lem := uniqueness_modulo_neutral_form js j1 j2; subst lem
+  replace j4 := stable_type_match_refl_inversion j4
+  have lem := prefix_type_match_forced_refl j4 j5; subst lem
+  apply j3
 case _ hd tl ih =>
   cases j4
   case _ h =>
@@ -58,29 +59,29 @@ case _ hd tl ih =>
       replace j2 := inversion_apply_spine j2
       cases j2; case _ W j2 =>
       cases j2; case _ j2 =>
+      cases j2; case _ j2 _ =>
       cases j2; case _ C D q1 q2 q3 =>
-        sorry
-        -- have lem := uniqueness_of_types j1 q1
-        -- subst lem; unfold ValidHeadVariable at h
-        -- simp at h
+        have lem := uniqueness_modulo_neutral_form js j1 q1
+        subst lem; unfold ValidHeadVariable at h
+        simp at h
     case _ =>
       replace j2 := inversion_apply_spine j2
       cases j2; case _ W j2 =>
       cases j2; case _ j2 =>
+      cases j2; case _ j2 _ =>
       cases j2; case _ C D q1 q2 q3 =>
-        sorry
-        -- have lem := uniqueness_of_types j1 q1
-        -- subst lem; unfold ValidHeadVariable at h
-        -- simp at h
+        have lem := uniqueness_modulo_neutral_form js j1 q1
+        subst lem; unfold ValidHeadVariable at h
+        simp at h
     case _ =>
       replace j2 := inversion_apply_spine j2
       cases j2; case _ W j2 =>
       cases j2; case _ j2 =>
+      cases j2; case _ j2 _ =>
       cases j2; case _ A q1 q2 =>
-        sorry
-        -- have lem := uniqueness_of_types j1 q2
-        -- subst lem; unfold ValidHeadVariable at h
-        -- simp at h
+        have lem := uniqueness_modulo_neutral_form js j1 q2
+        subst lem; unfold ValidHeadVariable at h
+        simp at h
   case _ U V _ h1 =>
     cases j5
     case _ h2 =>
@@ -92,34 +93,34 @@ case _ hd tl ih =>
         have lem0 := inversion_apply_spine j2
         cases lem0; case _ W lem0 =>
         cases lem0; case _ lem0 =>
+        cases lem0; case _ lem0 _ =>
         cases lem0; case _ q1 q2 q3 =>
-          sorry
-          -- have lem0 := uniqueness_of_types j1 q1
-          -- injection lem0 with _ e1 e2; subst e1; subst e2
-          -- have lem1 : Γ ⊢ q : V := q2
-          -- have lem2 := Judgment.app j3 lem1 rfl
-          -- have lem3 := Judgment.app j1 lem1 rfl
-          -- replace h1 := stable_type_match_beta q (by unfold Frame.is_stable; simp) h1
-          -- replace h2 := prefix_type_match_beta q (by unfold Frame.is_stable; simp) h2
-          -- simp at h1; simp at h2
-          -- replace ih := ih lem3 j2 lem2 h1 h2
-          -- apply ih
+          have lem0 := uniqueness_modulo_neutral_form js j1 q1
+          injection lem0 with _ e1 e2; subst e1; subst e2
+          have lem1 : Γ ⊢ q : V := q2
+          have lem2 := Judgment.app j3 lem1 rfl
+          have lem3 := Judgment.app j1 lem1 rfl
+          replace h1 := stable_type_match_beta q (by unfold Frame.is_stable; simp) h1
+          replace h2 := prefix_type_match_beta q (by unfold Frame.is_stable; simp) h2
+          simp at h1; simp at h2
+          apply @ih x (sp ++ [(.term, q)]) _ _ _ _ _ _ _ _ lem3 j2 lem2 h1 h2
+          simp; rw [Option.bind_eq_some]; simp; apply js
       case _ =>
         replace j2 := inversion_apply_spine j2
         cases j2; case _ W j2 =>
         cases j2; case _ j2 =>
+        cases j2; case _ j2 _ =>
         cases j2; case _ C D q1 q2 q3 =>
-          sorry
-          -- have lem := uniqueness_of_types j1 q1
-          -- injection lem with e; injection e
+        have lem := uniqueness_modulo_neutral_form js j1 q1
+        injection lem with e; injection e
       case _ =>
         replace j2 := inversion_apply_spine j2
         cases j2; case _ W j2 =>
         cases j2; case _ j2 =>
+        cases j2; case _ j2 _ =>
         cases j2; case _ C q1 q2 =>
-          sorry
-          -- have lem := uniqueness_of_types j1 q2
-          -- injection lem
+        have lem := uniqueness_modulo_neutral_form js j1 q2
+        injection lem
   case _ U V _ h1 =>
     cases j5
     case _ h2 =>
@@ -131,34 +132,34 @@ case _ hd tl ih =>
         replace j2 := inversion_apply_spine j2
         cases j2; case _ W j2 =>
         cases j2; case _ j2 =>
+        cases j2; case _ j2 _ =>
         cases j2; case _ C D q1 q2 q3 =>
-          sorry
-          -- have lem := uniqueness_of_types j1 q1
-          -- injection lem with e; injection e
+        have lem := uniqueness_modulo_neutral_form js j1 q1
+        injection lem with e; injection e
       case _ =>
         have lem0 := inversion_apply_spine j2
         cases lem0; case _ W lem0 =>
         cases lem0; case _ lem0 =>
+        cases lem0; case _ lem0 _ =>
         cases lem0; case _ q1 q2 q3 =>
-          sorry
-          -- have lem0 := uniqueness_of_types j1 q1
-          -- injection lem0 with _ e1 e2; subst e1; subst e2
-          -- have lem1 : Γ ⊢ q : U := q2
-          -- have lem2 := Judgment.appt j3 lem1 rfl
-          -- have lem3 := Judgment.appt j1 lem1 rfl
-          -- replace h1 := stable_type_match_beta q (by unfold Frame.is_stable; simp) h1
-          -- replace h2 := prefix_type_match_beta q (by unfold Frame.is_stable; simp) h2
-          -- simp at h1; simp at h2
-          -- replace ih := ih lem3 j2 lem2 h1 h2
-          -- apply ih
+        have lem0 := uniqueness_modulo_neutral_form js j1 q1
+        injection lem0 with _ e1 e2; subst e1; subst e2
+        have lem1 : Γ ⊢ q : U := q2
+        have lem2 := Judgment.appt j3 lem1 rfl
+        have lem3 := Judgment.appt j1 lem1 rfl
+        replace h1 := stable_type_match_beta q (by unfold Frame.is_stable; simp) h1
+        replace h2 := prefix_type_match_beta q (by unfold Frame.is_stable; simp) h2
+        simp at h1; simp at h2
+        apply @ih x (sp ++ [(.type, q)]) _ _ _ _ _ _ _ _ lem3 j2 lem2 h1 h2
+        simp; rw [Option.bind_eq_some]; simp; apply js
       case _ =>
         replace j2 := inversion_apply_spine j2
         cases j2; case _ W j2 =>
         cases j2; case _ j2 =>
+        cases j2; case _ j2 _ =>
         cases j2; case _ C q1 q2 =>
-          sorry
-          -- have lem := uniqueness_of_types j1 q2
-          -- injection lem
+        have lem := uniqueness_modulo_neutral_form js j1 q2
+        injection lem
 
 theorem preservation_prefix_match {p s t : Term} :
   Γ ⊢ p : A ->
@@ -173,331 +174,666 @@ theorem preservation_prefix_match {p s t : Term} :
 := by
 intro j1 j2 j3 j4 j5 j6 j7 j8
 replace j6 := prefix_equal_law j6; subst j6
-replace j7 := Term.neutral_form_law j7; subst j7
+have h7 := Term.neutral_form_law j7; subst h7
 replace j8 := Term.neutral_form_law j8; subst j8
 rw [Term.apply_spine_compose] at j2
-apply preservation_prefix_match_lemma j1 j2 j3 j4 j5
+apply preservation_prefix_match_lemma (Eq.symm j7) j1 j2 j3 j4 j5
+
+theorem type_choice_list :
+  t = List.foldl (·⊕·) a tl ->
+  Γ ⊢ A : ★ ->
+  Γ ⊢ a : A ->
+  (∀ x, x ∈ tl -> Γ ⊢ x : A) ->
+  Γ ⊢ t : A
+:= by
+intro h1 h2 h3 h4
+induction tl generalizing t Γ A a <;> simp at *
+subst h1; assumption
+case _ hd tl ih =>
+  apply @ih t (a ⊕ hd) Γ A h1 h2 _ h4.2
+  apply Judgment.choice _ h2 h3 h4.1
+  constructor; apply judgment_ctx_wf h2
 
 @[simp]
 abbrev PreservationLemmaType (Γ : Ctx Term) : (v : JudgmentVariant) -> JudgmentArgs v -> Prop
 | .prf => λ (t, A) => ∀ {t'}, Red Γ t t' -> Γ ⊢ t' : A
 | .wf => λ () => True
 
-theorem preservation_lemma : Judgment v Γ ix -> PreservationLemmaType Γ v ix := by sorry
--- intro j
--- induction j <;> simp at *
--- all_goals (intro ℓ t' r rin)
--- any_goals (solve | cases r <;> simp at *)
--- case _ j1 j2 j3 j4 ih1 ih2 ih3 ih4 =>
---   cases r <;> simp at *; subst rin
---   have lem := beta_term j3 j2; simp at lem
---   apply lem
--- case _ wf j _ =>
---   cases r <;> try simp at *
---   case _ x sp ℓ i1 i2 i3 i4 =>
---     cases i4; case _ e1 e2 =>
---       subst e1; subst e2
---       unfold Frame.is_openm at i1; split at i1 <;> simp at *
---       case _ f T h =>
---         rw [h] at j; unfold Frame.get_type at j; simp at j
---         subst i3; subst j; subst i2
---         apply (ctx_get_instance_well_typed wf h rin).2
---   case _ A x sp t h1 h2 =>
---     cases h2; case _ h2 h3 =>
---       subst h2; subst h3; unfold Term.apply_spine at rin
---       subst rin; rw [<-h1] at j; unfold Frame.get_type at j; simp at j
---       subst j
---       apply (ctx_get_term_well_typed wf (Eq.symm h1)).2
--- case appk j1 j2 ih1 ih2 =>
---   cases r
---   case _ x sp ℓ' i1 i2 i3 i4 =>
---     simp at i3; replace i3 := Eq.symm i3
---     rw [Option.bind_eq_some] at i3; simp at i3
---     cases i3; case _ x' i3 =>
---     cases i3; case _ sp' i3 =>
---     cases i3; case _ h1 h2 =>
---     cases h2; case _ h2 h3 =>
---       subst h2; subst h3; subst i4
---       simp at rin; cases rin; case _ w rin =>
---       cases rin; case _ q1 q2 =>
---         subst q2; subst i2
---         have lem := preservation_inst_lemma j1 h1 i1 q1
---         rw [Term.apply_spine_peel_kind]; constructor
---         apply lem; apply j2
---   case _ T x sp t i1 i2 =>
---     simp at i2; replace i2 := Eq.symm i2
---     rw [Option.bind_eq_some] at i2; simp at i2
---     cases i2; case _ x' i2 =>
---     cases i2; case _ sp' i2 =>
---     cases i2; case _ h1 h2 =>
---     cases h2; case _ h2 h3 =>
---       subst h2; subst h3; simp at rin; subst rin
---       have lem := preservation_letterm_lemma j1 h1 i1
---       rw [Term.apply_spine_peel_kind]; constructor
---       apply lem; apply j2
--- case ite j1 j2 j3 j4 j5 j6 j7 j8 j9 j10 ih1 ih2 ih3 ih4 ih5 ih6 =>
---   cases r <;> try simp at *
---   case _ x sp sp' ξ h1 h2 h3 h4 =>
---     subst rin
---     apply preservation_prefix_match j1 j2 j4 j7 j8 h1 h3 h4
---   case _ => subst rin; apply j10
---   case _ ℓ' r h =>
---     subst h; simp at rin
---     cases rin; case _ w h =>
---     cases h; case _ h1 h2 =>
---       subst h2; replace ih2 := ih2 r h1
---       apply Judgment.ite j1 ih2 j3 j4 j5 j6 j7 j8 j9 j10
--- case guard j1 j2 j3 j4 j5 j6 j7 j8 j9 ih1 ih2 ih3 ih4 ih5 =>
---   cases r <;> try simp at *
---   case _ x sp sp' ξ h1 h2 h3 =>
---     subst rin
---     apply preservation_prefix_match j1 j2 j4 j7 j8 h1 h2 h3
---   case _ ℓ' r h =>
---     subst h; simp at rin
---     cases rin; case _ w h =>
---     cases h; case _ h1 h2 =>
---       subst h2; replace ih2 := ih2 r h1
---       apply Judgment.guard j1 ih2 j3 j4 j5 j6 j7 j8 j9
--- case app a _ j1 j2 j3 ih1 ih2 =>
---   cases r
---   case _ =>
---     simp at rin; subst rin
---     cases j1; case _ j4 j5 j6 =>
---       have lem := beta_type j6 j2
---       subst j3; apply lem
---   case _ x sp ℓ' i1 i2 i3 i4 =>
---     simp at i3; replace i3 := Eq.symm i3
---     rw [Option.bind_eq_some] at i3; simp at i3
---     cases i3; case _ x' i3 =>
---     cases i3; case _ sp' i3 =>
---     cases i3; case _ h1 h2 =>
---     cases h2; case _ h2 h3 =>
---       subst h2; subst h3; subst i4
---       simp at rin; cases rin; case _ w rin =>
---       cases rin; case _ q1 q2 =>
---         subst q2; subst i2
---         have lem := preservation_inst_lemma j1 h1 i1 q1
---         rw [Term.apply_spine_peel_term]; constructor
---         apply lem; apply j2; apply j3
---   case _ T x sp t i1 i2 =>
---     simp at i2; replace i2 := Eq.symm i2
---     rw [Option.bind_eq_some] at i2; simp at i2
---     cases i2; case _ x' i2 =>
---     cases i2; case _ sp' i2 =>
---     cases i2; case _ h1 h2 =>
---     cases h2; case _ h2 h3 =>
---       subst h2; subst h3; simp at rin; subst rin
---       have lem := preservation_letterm_lemma j1 h1 i1
---       rw [Term.apply_spine_peel_term]; constructor
---       apply lem; apply j2; apply j3
---   case _ ℓ' r h =>
---     subst h; simp at rin
---     cases rin; case _ f' h =>
---     cases h; case _ h1 h2 =>
---       subst h2; constructor
---       apply ih1 r h1; apply j2; apply j3
--- case appt j1 j2 j3 ih1 ih2 =>
---   cases r
---   case _ =>
---     simp at rin; subst rin
---     cases j1; case _ j4 j5 j6 =>
---       have lem := beta_kind j6 j2
---       subst j3; apply lem
---   case _ x sp ℓ' i1 i2 i3 i4 =>
---     simp at i3; replace i3 := Eq.symm i3
---     rw [Option.bind_eq_some] at i3; simp at i3
---     cases i3; case _ x' i3 =>
---     cases i3; case _ sp' i3 =>
---     cases i3; case _ h1 h2 =>
---     cases h2; case _ h2 h3 =>
---       subst h2; subst h3; subst i4
---       simp at rin; cases rin; case _ w rin =>
---       cases rin; case _ q1 q2 =>
---         subst q2; subst i2
---         have lem := preservation_inst_lemma j1 h1 i1 q1
---         rw [Term.apply_spine_peel_type]; constructor
---         apply lem; apply j2; apply j3
---   case _ T x sp t i1 i2 =>
---     simp at i2; replace i2 := Eq.symm i2
---     rw [Option.bind_eq_some] at i2; simp at i2
---     cases i2; case _ x' i2 =>
---     cases i2; case _ sp' i2 =>
---     cases i2; case _ h1 h2 =>
---     cases h2; case _ h2 h3 =>
---       subst h2; subst h3; simp at rin; subst rin
---       have lem := preservation_letterm_lemma j1 h1 i1
---       rw [Term.apply_spine_peel_type]; constructor
---       apply lem; apply j2; apply j3
---   case _ ℓ' r h =>
---     subst h; simp at rin
---     cases rin; case _ f' h =>
---     cases h; case _ h1 h2 =>
---       subst h2; constructor
---       apply ih1 r h1; apply j2; apply j3
--- case _ j1 j2 ih1 ih2 =>
---   cases r <;> try simp at *
---   case _ =>
---     subst rin; cases j2; case _ =>
---       apply j1
---   case _ ℓ' r' h =>
---     subst h; simp at rin
---     cases rin; case _ z h =>
---     cases h; case _ h1 h2 =>
---       subst h2; constructor
---       apply j1; apply ih2 r' h1
--- case _ j ih =>
---   cases r <;> try simp at *
---   case _ =>
---     subst rin; cases j; case _ j1 j2 =>
---       constructor; apply j1; apply j2
---   case _ ℓ' r' h =>
---     subst h; simp at rin
---     cases rin; case _ z h =>
---     cases h; case _ h1 h2 =>
---       subst h2; constructor
---       apply ih r' h1
--- case seq j1 j2 ih1 ih2 =>
---   cases r <;> try simp at *
---   case _ =>
---     have lem := uniqueness_of_types j1 j2
---     injection lem with _ e1 e2; subst e1; subst e2
---     cases j1; case _ j1 j3 =>
---     subst rin; apply Judgment.refl j1 j3
---   case _ ℓ' r h =>
---     subst h; simp at rin
---     cases rin; case _ z h =>
---     cases h; case _ h1 h2 =>
---       subst h2; constructor
---       apply ih1 r h1; apply j2
---   case _ ℓ' r h =>
---     subst h; simp at rin
---     cases rin; case _ z h =>
---     cases h; case _ h1 h2 =>
---       subst h2; constructor
---       apply j1; apply ih2 r h1
--- case _ Γ A K1 K2 B t1 C D t2 j1 j2 j3 j4 j5 j6 ih1 ih2 ih3 ih4 ih5 ih6 =>
---   cases r <;> try simp at *
---   case _ =>
---     subst rin
---     cases j3; case _ K1' q1 q2 =>
---     cases j6; case _ K2' w1 w2 =>
---       have lem0 := classification_lemma j2; simp at lem0
---       have lem : Γ ⊢ (A `@k C) : K2 := by
---         constructor; apply j2; apply j5
---       apply Judgment.refl _ lem
---       cases lem0
---       case _ lem0 =>
---         cases lem0; case _ w1 w2 => apply w2
---       case _ lem0 =>
---         cases lem0; case _ K3 w1 w2 =>
---         cases w2.2; cases w2.1
---   case _ ℓ' r h =>
---     subst h; simp at rin
---     cases rin; case _ z h =>
---     cases h; case _ h1 h2 =>
---       subst h2; constructor
---       apply j1; apply j2; apply ih3 r h1
---       apply j4; apply j5; apply j6
---   case _ ℓ' r h =>
---     subst h; simp at rin
---     cases rin; case _ z h =>
---     cases h; case _ h1 h2 =>
---       subst h2; constructor
---       apply j1; apply j2; apply j3
---       apply j4; apply j5; apply ih6 r h1
--- case _ Γ A B t1 C D t2 j1 j2 j3 j4 j5 j6 ih1 ih2 ih3 ih4 ih5 ih6 =>
---   cases r <;> try simp at *
---   case _ =>
---     subst rin
---     cases j3; case _ K1 q1 q2 =>
---     cases j6; case _ K2 w1 w2 =>
---       have lem : Γ ⊢ (A -t> C) : ★ := by
---         constructor; apply j2; apply j5
---       apply Judgment.refl _ lem; constructor
---       apply judgment_ctx_wf j1
---   case _ ℓ' r h =>
---     subst h; simp at rin
---     cases rin; case _ z h =>
---     cases h; case _ h1 h2 =>
---       subst h2; constructor
---       apply j1; apply j2; apply ih3 r h1
---       apply j4; apply j5; apply j6
---   case _ ℓ' r h =>
---     subst h; simp at rin
---     cases rin; case _ z h =>
---     cases h; case _ h1 h2 =>
---       subst h2; constructor
---       apply j1; apply j2; apply j3
---       apply j4; apply j5; apply ih6 r h1
--- case _ j1 j2 j3 ih1 ih2 ih3 =>
---   cases r <;> try simp at *
---   case _ =>
---     subst rin
---     cases j3; case _ K1 q1 q2 =>
---     apply Judgment.refl _ j1
---     have lem := classification_lemma j1; simp at lem
---     cases lem
---     case _ lem => apply lem
---     case _ lem =>
---       cases lem; case _ K3 lem =>
---         cases lem.2; cases lem.1
---   case _ ℓ' r h =>
---     subst h; simp at rin
---     cases rin; case _ z h =>
---     cases h; case _ h1 h2 =>
---       subst h2; constructor
---       apply j1; apply j2; apply ih3 r h1
--- case _ j1 j2 j3 j4 ih1 ih2 ih3 ih4 =>
---   cases r <;> try simp at *
---   case _ =>
---     subst rin
---     cases j4; case _ K1 q1 q2 =>
---       apply Judgment.refl j1 j2
---   case _ ℓ' r h =>
---     subst h; simp at rin
---     cases rin; case _ z h =>
---     cases h; case _ h1 h2 =>
---       subst h2; constructor
---       apply j1; apply j2; apply j3
---       apply ih4 r h1
--- case _ j1 j2 j3 ih1 ih2 ih3 =>
---   cases r <;> try simp at *
---   case _ =>
---     subst rin
---     cases j3; case _ K1 q1 q2 =>
---       apply Judgment.refl _ j2; constructor
---       apply judgment_ctx_wf j1
---   case _ ℓ' r h =>
---     subst h; simp at rin
---     cases rin; case _ z h =>
---     cases h; case _ h1 h2 =>
---       subst h2; constructor
---       apply j1; apply j2; apply ih3 r h1
--- case _ j1 j2 j3 j4 j5 j6 ih1 ih2 ih3 ih4 =>
---   cases r <;> try simp at *
---   case _ =>
---     subst rin
---     cases j1; case _ K1 q1 q2 =>
---     cases j4; case _ K2 w1 w2 =>
---     cases q2; case _ i1 i2 =>
---       replace i2 := beta_kind i2 j3; simp at i2
---       subst j5; subst j6
---       apply Judgment.refl _ i2; constructor
---       apply judgment_ctx_wf j2
---   case _ ℓ' r h =>
---     subst h; simp at rin
---     cases rin; case _ z h =>
---     cases h; case _ h1 h2 =>
---       subst h2; constructor
---       apply ih1 r h1; apply j2; apply j3
---       apply j4; apply j5; apply j6
---   case _ ℓ' r h =>
---     subst h; simp at rin
---     cases rin; case _ z h =>
---     cases h; case _ h1 h2 =>
---       subst h2; constructor
---       apply j1; apply j2; apply j3
---       apply ih4 r h1; apply j5; apply j6
+theorem preservation_lemma : Judgment v Γ ix -> PreservationLemmaType Γ v ix := by
+intro j
+induction j <;> simp at *
+all_goals (intro t' r)
+any_goals (solve | cases r <;> simp at *)
+case letterm j1 j2 j3 j4 ih1 ih2 ih3 ih4 =>
+  cases r
+  case _ =>
+    have lem := beta_term j3 j2
+    simp at lem; apply lem
+  case _ h _ => cases h
+  case _ h => cases h
+case var Γ x T j1 j2 _ =>
+  cases r
+  case _ i sp tl tl' h1 h2 h3 h4 h5 =>
+    simp at h4; cases h4; case _ e1 e2 =>
+      subst e1; subst e2
+      simp at h1; subst h1
+      have lem1 := frame_wf_by_index i j1
+      have lem2 := frame_wf_openm_implies_type T lem1 j2 h2
+      have lem3 : Γ ⊢ `0 : T := by
+        apply Judgment.empty _ lem2
+        constructor; apply judgment_ctx_wf lem2
+      apply type_choice_list h5 lem2 lem3
+      intro x h; subst h3
+      replace h := get_instances_sound h
+      cases h; case _ y h =>
+      have lem := frame_wf_by_index y j1
+      rw [h] at lem
+      cases lem; case _ T' q1 q2 =>
+      rw [<-q1] at j2
+      unfold Frame.get_type at j2; simp at j2
+      subst j2; apply q2
+  case _ T' i sp t h1 h2 =>
+    simp at h2; cases h2; case _ e1 e2 =>
+      subst e1; subst e2; simp
+      have lem := frame_wf_by_index i j1
+      rw [<-h1] at lem
+      cases lem; case _ q1 q2 =>
+      rw [<-h1] at j2; unfold Frame.get_type at j2
+      simp at j2; subst j2; apply q2
+case appk Γ f A B a j1 j2 ih1 ih2 =>
+  cases r
+  case _ x sp tl tl' h1 h2 h3 h4 h5 =>
+    have lem := frame_wf_by_index x (judgment_ctx_wf j1)
+    have lem2 := Frame.is_openm_destruct h2
+    cases lem2; case _ T lem2 =>
+    rw [lem2] at lem; cases lem; case _ q1 =>
+    have lem3 := Term.neutral_form_law h4
+    have j3 := Judgment.appk j1 j2
+    rw [<-lem3] at j3
+    have lem4 := inversion_apply_spine j3
+    cases lem4; case _ T' lem4 =>
+    cases lem4.2.1; case _ h1 h2 =>
+    rw [lem2] at h2; unfold Frame.get_type at h2
+    simp at h2; subst h2
+    have lem5 := classification_lemma j1; simp at lem5
+    cases lem5; case inr lem5 =>
+      cases lem5; case _ K lem5 =>
+      cases lem5.2; cases lem5.1
+    case _ lem5 =>
+    cases lem5; case _ w1 w2 =>
+      have lem6 := lem4.2.2 _ w2
+      have lem7 := kind_shape lem6 rfl
+      have lem8 := type_shape q1 (by constructor)
+      exfalso; apply Term.is_kind_disjoint_is_type lem7 lem8
+  case _ T x sp t h1 h2 =>
+    apply preservation_letterm_lemma _ (Eq.symm h2) h1
+    apply Judgment.appk j1 j2
+  case _ h _ => cases h
+  case _ h _ => cases h
+  case _ h => cases h
+  case _ h => cases h
+  case _ h _ => cases h
+  case _ h _ => cases h
+case ite j1 j2 j3 j4 j5 j6 j7 j8 j9 j10 ih1 ih2 ih3 ih4 ih5 ih6 =>
+  cases r
+  case _ h1 h2 h3 h4 =>
+    apply preservation_prefix_match j1 j2 j4 j7 j8 h1 h3 h4
+  case _ => apply j10
+  case _ h _ => cases h
+  case _ h => cases h
+  case _ r => apply Judgment.ite j1 (ih2 r) j3 j4 j5 j6 j7 j8 j9 j10
+  case _ =>
+    apply Judgment.empty _ j9
+    constructor; apply judgment_ctx_wf j1
+  case _ =>
+    cases j2; case _ q1 q2 q3 q4 =>
+    apply Judgment.choice _ j9
+    apply Judgment.ite j1 q3 j3 j4 j5 j6 j7 j8 j9 j10
+    apply Judgment.ite j1 q4 j3 j4 j5 j6 j7 j8 j9 j10
+    constructor; apply judgment_ctx_wf j1
+case guard j1 j2 j3 j4 j5 j6 j7 j8 j9 ih1 ih2 ih3 ih4 ih5 =>
+  cases r
+  case _ h1 h2 h3 =>
+    apply preservation_prefix_match j1 j2 j4 j7 j8 h1 h2 h3
+  case _ =>
+    apply Judgment.empty _ j9
+    constructor; apply judgment_ctx_wf j1
+  case _ h _ => cases h
+  case _ h => cases h
+  case _ r => apply Judgment.guard j1 (ih2 r) j3 j4 j5 j6 j7 j8 j9
+  case _ =>
+    apply Judgment.empty _ j9
+    constructor; apply judgment_ctx_wf j1
+  case _ =>
+    cases j2; case _ q1 q2 q3 q4 =>
+    apply Judgment.choice _ j9
+    apply Judgment.guard j1 q3 j3 j4 j5 j6 j7 j8 j9
+    apply Judgment.guard j1 q4 j3 j4 j5 j6 j7 j8 j9
+    constructor; apply judgment_ctx_wf j1
+case app Γ f A B a B' j1 j2 j3 ih1 ih2 =>
+  have lem : Γ ⊢ (A -t> B) : ★ := by
+    have lem := classification_lemma j1; simp at lem
+    cases lem; case _ lem => cases lem
+    case _ lem =>
+    cases lem; case _ K lem =>
+    cases lem.2; apply lem.2
+  cases lem; case _ lem1 lem2 =>
+  have lem3 : Γ ⊢ B' : ★ := by
+    have lem := beta_empty a lem2
+    subst j3; simp at lem; apply lem
+  have lem4 : Γ ⊢ `0 : B' := by
+    apply Judgment.empty _ lem3
+    constructor; apply judgment_ctx_wf lem1
+  cases r
+  case _ =>
+    cases j1; case _ q1 q2 q3 =>
+    have lem := beta_type q3 j2
+    subst j3; apply lem
+  case _ x sp tl tl' h1 h2 h3 h4 h5 =>
+    apply type_choice_list h5 lem3 lem4; clear h5
+    intro y h6; subst h3; subst h1; simp at h6
+    cases h6; case _ w h3 =>
+    cases h3; case _ h3 h5 =>
+    replace h5 := Eq.symm h5; subst h5
+    have lem5 := get_instances_sound h3
+    cases lem5; case _ j lem5 =>
+    simp at h4; replace h4 := Option.bind_eq_some.1 (Eq.symm h4)
+    cases h4; case _ q h4 =>
+    cases q; case _ z sp' =>
+    simp at h4; cases h4; case _ h4 h5 =>
+    cases h5; case _ h5 h6 =>
+    subst h5; replace h6 := Eq.symm h6; subst h6
+    rw [Term.apply_spine_peel_term]
+    apply Judgment.app _ j2 j3
+    apply preservation_inst_lemma j1 h4 h2 h3
+  case _ T x sp t h1 h2 =>
+    apply preservation_letterm_lemma _ (Eq.symm h2) h1
+    apply Judgment.app j1 j2 j3
+  case _ r => apply Judgment.app (ih1 r) j2 j3
+  case _ h _ => cases h
+  case _ =>
+    cases j1; case _ j1 =>
+    cases j1; case _ q1 q2 q3 =>
+    have lem := beta_empty a q2
+    subst j3; simp at lem
+    apply Judgment.empty _ lem
+    constructor; apply judgment_ctx_wf lem
+  case _ h => cases h
+  case _ =>
+    cases j1; case _ q1 q2 q3 =>
+    cases q1; case _ q1 q4 q5 =>
+    have lem := beta_empty a q4; simp at lem
+    subst j3; apply Judgment.choice _ lem
+    apply Judgment.app q2 j2 rfl
+    apply Judgment.app q3 j2 rfl
+    constructor; apply judgment_ctx_wf q1
+  case _ h _ => cases h
+case appt Γ f A B a B' j1 j2 j3 ih1 ih2 =>
+  have lem : Γ ⊢ ∀[A] B : ★ := by
+    have lem := classification_lemma j1; simp at lem
+    cases lem; case _ lem => cases lem
+    case _ lem =>
+    cases lem; case _ K lem =>
+    cases lem.2; apply lem.2
+  cases lem; case _ lem1 lem2 =>
+  have lem3 : Γ ⊢ B' : ★ := by
+    have lem := beta_kind lem2 j2
+    subst j3; simp at lem; apply lem
+  have lem4 : Γ ⊢ `0 : B' := by
+    apply Judgment.empty _ lem3
+    constructor; apply judgment_ctx_wf lem1
+  cases r
+  case _ =>
+    cases j1; case _ q1 q2 q3 =>
+    have lem := beta_kind q3 j2
+    subst j3; apply lem
+  case _ x sp tl tl' h1 h2 h3 h4 h5 =>
+    apply type_choice_list h5 lem3 lem4; clear h5
+    intro y h6; subst h3; subst h1; simp at h6
+    cases h6; case _ w h3 =>
+    cases h3; case _ h3 h5 =>
+    replace h5 := Eq.symm h5; subst h5
+    have lem5 := get_instances_sound h3
+    cases lem5; case _ j lem5 =>
+    simp at h4; replace h4 := Option.bind_eq_some.1 (Eq.symm h4)
+    cases h4; case _ q h4 =>
+    cases q; case _ z sp' =>
+    simp at h4; cases h4; case _ h4 h5 =>
+    cases h5; case _ h5 h6 =>
+    subst h5; replace h6 := Eq.symm h6; subst h6
+    rw [Term.apply_spine_peel_type]
+    apply Judgment.appt _ j2 j3
+    apply preservation_inst_lemma j1 h4 h2 h3
+  case _ T x sp t h1 h2 =>
+    apply preservation_letterm_lemma _ (Eq.symm h2) h1
+    apply Judgment.appt j1 j2 j3
+  case _ r => apply Judgment.appt (ih1 r) j2 j3
+  case _ h _ => cases h
+  case _ =>
+    cases j1; case _ j1 =>
+    cases j1; case _ q1 q2 q3 =>
+    have lem := beta_kind q2 j2
+    subst j3; simp at lem
+    apply Judgment.empty _ lem
+    constructor; apply judgment_ctx_wf q1
+  case _ h => cases h
+  case _ =>
+    cases j1; case _ q1 q2 q3 =>
+    cases q1; case _ q1 q4 q5 =>
+    have lem := beta_kind q4 j2; simp at lem
+    subst j3; apply Judgment.choice _ lem3
+    apply Judgment.appt q2 j2 rfl
+    apply Judgment.appt q3 j2 rfl
+    constructor; apply judgment_ctx_wf q2
+  case _ h _ => cases h
+case cast j1 j2 ih1 ih2 =>
+  have lem1 := classification_lemma j2; simp at lem1
+  cases lem1; case _ lem1 => cases lem1
+  case _ lem1 =>
+  cases lem1; case _ K lem1 =>
+  cases lem1.2; case _ q1 q2 q3 =>
+  cases r
+  case _ => cases j2; apply j1
+  case _ h _ => cases h
+  case _ h => cases h
+  case _ h _ => cases h
+  case _ r => apply Judgment.cast j1 (ih2 r)
+  case _ h => cases h
+  case _ => apply Judgment.empty q1 q3
+  case _ h _ => cases h
+  case _ =>
+    cases j2; case _ w1 w2 w3 w4 =>
+    apply Judgment.choice q1 q3
+    apply Judgment.cast j1 w3
+    apply Judgment.cast j1 w4
+case sym j ih =>
+  cases r
+  case _ =>
+    cases j; case _ j1 j2 =>
+    apply Judgment.refl j1 j2
+  case _ h _ => cases h
+  case _ h => cases h
+  case _ r => apply Judgment.sym (ih r)
+  case _ =>
+    cases j; case _ j1 j2 =>
+    cases j2; case _ q1 q2 q3 =>
+    apply Judgment.empty j1
+    apply Judgment.eq q1 q3 q2
+  case _ =>
+    cases j; case _ q1 q2 q3 q4 =>
+    apply Judgment.choice q1 _
+    apply Judgment.sym q3
+    apply Judgment.sym q4
+    cases q2; case _ w1 w2 w3 =>
+    apply Judgment.eq w1 w3 w2
+case seq j1 j2 ih1 ih2 =>
+  cases r
+  case _ =>
+    cases j1; case _ q1 q2 =>
+    cases j2
+    apply Judgment.refl q1 q2
+  case _ h _ => cases h
+  case _ h => cases h
+  case _ r => apply Judgment.seq (ih1 r) j2
+  case _ r => apply Judgment.seq j1 (ih2 r)
+  case _ =>
+    cases j1; case _ q1 q2 =>
+    cases q2; case _ q2 q3 q4 =>
+    have lem := classification_lemma j2 <;> simp at lem
+    cases lem; case _ lem => cases lem
+    case _ lem =>
+    cases lem; case _ K lem =>
+    cases lem.2; case _ w1 w2 w3 =>
+    apply Judgment.empty lem.1
+    apply Judgment.eq q2 q3 w3
+  case _ =>
+    cases j2; case _ q1 q2 =>
+    cases q2; case _ q2 q3 q4 =>
+    have lem := classification_lemma j1 <;> simp at lem
+    cases lem; case _ lem => cases lem
+    case _ lem =>
+    cases lem; case _ K lem =>
+    cases lem.2; case _ w1 w2 w3 =>
+    apply Judgment.empty q1
+    apply Judgment.eq q2 w2 q4
+  case _ =>
+    cases j1; case _ q1 q2 q3 q4 =>
+    cases q2; case _ q2 q5 q6 =>
+    have lem := classification_lemma j2 <;> simp at lem
+    cases lem; case _ lem => cases lem
+    case _ lem =>
+    cases lem; case _ K lem =>
+    cases lem.2; case _ w1 w2 w3 =>
+    apply Judgment.choice q1
+    apply Judgment.eq q2 q5 w3
+    apply Judgment.seq q3 j2
+    apply Judgment.seq q4 j2
+  case _ =>
+    cases j2; case _ q1 q2 q3 q4 =>
+    cases q2; case _ q2 q5 q6 =>
+    have lem := classification_lemma j1 <;> simp at lem
+    cases lem; case _ lem => cases lem
+    case _ lem =>
+    cases lem; case _ K lem =>
+    cases lem.2; case _ w1 w2 w3 =>
+    apply Judgment.choice lem.1
+    apply Judgment.eq q2 w2 q6
+    apply Judgment.seq j1 q3
+    apply Judgment.seq j1 q4
+case appc j1 j2 ih1 ih2 =>
+  cases r
+  case _ =>
+    cases j1; case _ q1 q2 =>
+    cases q1; case _ q1 q3 =>
+    cases j2; case _ w1 w2 =>
+    apply Judgment.refl q3
+    apply Judgment.appk q2 w2
+  case _ h _ => cases h
+  case _ h => cases h
+  case _ r => apply Judgment.appc (ih1 r) j2
+  case _ r => apply Judgment.appc j1 (ih2 r)
+  case _ =>
+    cases j1; case _ q1 q2 =>
+    cases q2; case _ q2 q3 q4 =>
+    cases q2; case _ q2 q5 =>
+    have lem := classification_lemma j2; simp at lem
+    cases lem; case _ lem => cases lem
+    case _ lem =>
+    cases lem; case _ K lem =>
+    cases lem.2; case _ w1 w2 w3 =>
+    apply Judgment.empty q1
+    apply Judgment.eq q5
+    apply Judgment.appk q3 w2
+    apply Judgment.appk q4 w3
+  case _ =>
+    cases j2; case _ q1 q2 =>
+    cases q2; case _ q2 q3 q4 =>
+    have lem := classification_lemma j1; simp at lem
+    cases lem; case _ lem => cases lem
+    case _ lem =>
+    cases lem; case _ K lem =>
+    cases lem.2; case _ w1 w2 w3 =>
+    cases w1; case _ w1 w4 =>
+    apply Judgment.empty q1
+    apply Judgment.eq w4
+    apply Judgment.appk w2 q3
+    apply Judgment.appk w3 q4
+  case _ =>
+    cases j1; case _ q1 q2 q3 q4 =>
+    cases q2; case _ q2 q5 q6 =>
+    cases q2; case _ q2 q7 =>
+    have lem := classification_lemma j2; simp at lem
+    cases lem; case _ lem => cases lem
+    case _ lem =>
+    cases lem; case _ K lem =>
+    cases lem.2; case _ w1 w2 w3 =>
+    apply Judgment.choice q1
+    apply Judgment.eq q7
+    apply Judgment.appk q5 w2
+    apply Judgment.appk q6 w3
+    apply Judgment.appc q3 j2
+    apply Judgment.appc q4 j2
+  case _ =>
+    cases j2; case _ q1 q2 q3 q4 =>
+    cases q2; case _ q2 q5 q6 =>
+      have lem := classification_lemma j1; simp at lem
+      cases lem; case _ lem => cases lem
+      case _ lem =>
+      cases lem; case _ K lem =>
+      cases lem.2; case _ w1 w2 w3 =>
+      cases w1; case _ w1 w4 =>
+        apply Judgment.choice q1
+        apply Judgment.eq w4
+        apply Judgment.appk w2 q5
+        apply Judgment.appk w3 q6
+        apply Judgment.appc j1 q3
+        apply Judgment.appc j1 q4
+case arrowc j1 j2 ih1 ih2 =>
+  cases r
+  case _ =>
+    cases j1; case _ q1 q2 =>
+    cases j2; case _ w1 w2 =>
+    apply Judgment.refl q1
+    apply Judgment.arrow q2 w2
+  case _ h _ => cases h
+  case _ h => cases h
+  case _ r => apply Judgment.arrowc (ih1 r) j2
+  case _ r => apply Judgment.arrowc j1 (ih2 r)
+  case _ =>
+    cases j1; case _ q1 q2 =>
+    cases q2; case _ q2 q3 q4 =>
+    have lem := classification_lemma j2; simp at lem
+    cases lem; case _ lem => cases lem
+    case _ lem =>
+    cases lem; case _ K lem =>
+    cases lem.2; case _ w1 w2 w3 =>
+    apply Judgment.empty q1
+    apply Judgment.eq q1
+    apply Judgment.arrow q3 w2
+    apply Judgment.arrow q4 w3
+  case _ =>
+    cases j2; case _ q1 q2 =>
+    cases q2; case _ q2 q3 q4 =>
+    have lem := classification_lemma j1; simp at lem
+    cases lem; case _ lem => cases lem
+    case _ lem =>
+    cases lem; case _ K lem =>
+    cases lem.2; case _ w1 w2 w3 =>
+    apply Judgment.empty w1
+    apply Judgment.eq w1
+    apply Judgment.arrow w2 q3
+    apply Judgment.arrow w3 q4
+  case _ =>
+    cases j1; case _ q1 q2 q3 q4 =>
+    cases q2; case _ q2 q5 q6 =>
+    have lem := classification_lemma j2; simp at lem
+    cases lem; case _ lem => cases lem
+    case _ lem =>
+    cases lem; case _ K lem =>
+    cases lem.2; case _ w1 w2 w3 =>
+    apply Judgment.choice q2
+    apply Judgment.eq q2
+    apply Judgment.arrow q5 w2
+    apply Judgment.arrow q6 w3
+    apply Judgment.arrowc q3 j2
+    apply Judgment.arrowc q4 j2
+  case _ =>
+    cases j2; case _ q1 q2 q3 q4 =>
+    cases q2; case _ q2 q5 q6 =>
+    have lem := classification_lemma j1; simp at lem
+    cases lem; case _ lem => cases lem
+    case _ lem =>
+    cases lem; case _ K lem =>
+    cases lem.2; case _ w1 w2 w3 =>
+    apply Judgment.choice w1
+    apply Judgment.eq w1
+    apply Judgment.arrow w2 q5
+    apply Judgment.arrow w3 q6
+    apply Judgment.arrowc j1 q3
+    apply Judgment.arrowc j1 q4
+case fst j1 j2 j3 ih1 ih2 ih3 =>
+  cases r
+  case _ =>
+    cases j3; case _ q1 q2 =>
+    have lem := classification_lemma j1; simp at lem
+    cases lem; case inr lem =>
+      cases lem; case _ K lem =>
+      cases lem.2; cases lem.1
+    case _ lem =>
+      apply Judgment.refl lem j1
+  case _ h _ => cases h
+  case _ h => cases h
+  case _ h _ => cases h
+  case _ r => apply Judgment.fst j1 j2 (ih3 r)
+  case _ h => cases h
+  case _ =>
+    cases j3; case _ q1 q2 =>
+    cases q2; case _ q2 q3 q4 =>
+    cases q3; case _ K3 q3 q5 =>
+    cases q4; case _ K3 q4 q6 =>
+    have lem1 := classification_lemma j1; simp at lem1
+    cases lem1; case inr lem =>
+      cases lem; case _ K lem =>
+      cases lem.2; cases lem.1
+    case _ lem =>
+      have lem3 := type_shape j2 (kind_shape lem rfl)
+      have lem5 := uniqueness_of_kinds lem3 j2 q6
+      injection lem5 with _ e; subst e
+      apply Judgment.empty q1
+      apply Judgment.eq lem j1 q6
+  case _ h _ => cases h
+  case _ =>
+    cases j3; case _ q1 q2 q3 q4 =>
+    cases q2; case _ q2 q5 q6 =>
+    have lem1 := classification_lemma j1; simp at lem1
+    cases lem1; case inr lem =>
+      cases lem; case _ K lem =>
+      cases lem.2; cases lem.1
+    case _ lem1 =>
+      apply Judgment.choice q1
+      apply Judgment.eq lem1 j1 j2
+      apply Judgment.fst j1 j2 q3
+      apply Judgment.fst j1 j2 q4
+case snd j1 j2 j3 j4 ih1 ih2 ih3 ih4 =>
+  cases r
+  case _ =>
+    cases j4; case _ q1 q2 =>
+    apply Judgment.refl j1 j2
+  case _ h _ => cases h
+  case _ h => cases h
+  case _ h _ => cases h
+  case _ r => apply Judgment.snd j1 j2 j3 (ih4 r)
+  case _ h => cases h
+  case _ =>
+    apply Judgment.empty _
+    apply Judgment.eq j1 j2 j3
+    constructor; apply judgment_ctx_wf j1
+  case _ h _ => cases h
+  case _ =>
+    cases j4; case _ q1 q2 q3 q4 =>
+    cases q2; case _ q2 q5 q6 =>
+    apply Judgment.choice q1
+    apply Judgment.eq j1 j2 j3
+    apply Judgment.snd j1 j2 j3 q3
+    apply Judgment.snd j1 j2 j3 q4
+case allc j1 j2 ih1 ih2 =>
+  cases r
+  case _ =>
+    cases j2; case _ q1 q2 =>
+    apply Judgment.refl _
+    apply Judgment.allt j1 q2
+    constructor; apply judgment_ctx_wf j1
+  case _ h _ => cases h
+  case _ h => cases h
+  case _ h _ => cases h
+  case _ r => apply Judgment.allc j1 (ih2 r)
+  case _ h => cases h
+  case _ =>
+    cases j2; case _ q1 q2 =>
+    cases q2; case _ q2 q3 q4 =>
+    apply Judgment.empty _
+    apply Judgment.eq _
+    apply Judgment.allt j1 q3
+    apply Judgment.allt j1 q4
+    constructor; apply judgment_ctx_wf j1
+    constructor; apply judgment_ctx_wf j1
+  case _ h => cases h
+  case _ =>
+    cases j2; case _ q1 q2 q3 q4 =>
+    cases q2; case _ q2 q5 q6 =>
+    apply Judgment.choice _
+    apply Judgment.eq _
+    apply Judgment.allt j1 q5
+    apply Judgment.allt j1 q6
+    constructor; apply judgment_ctx_wf j1
+    apply Judgment.allc j1 q3
+    apply Judgment.allc j1 q4
+    constructor; apply judgment_ctx_wf j1
+case apptc j1 j2 j3 j4 ih1 ih2 =>
+  cases r
+  case _ =>
+    cases j1; case _ q1 q2 =>
+    cases j2; case _ q3 q4 =>
+    cases q2; case _ q2 q5 =>
+    subst j3; subst j4
+    apply Judgment.refl q3
+    apply beta_kind q5 q4
+  case _ h _ => cases h
+  case _ h => cases h
+  case _ r => apply Judgment.apptc (ih1 r) j2 j3 j4
+  case _ r => apply Judgment.apptc j1 (ih2 r) j3 j4
+  case _ =>
+    cases j1; case _ q1 q2 =>
+    cases q2; case _ q2 q3 q4 =>
+    cases q3; case _ w1 w2 =>
+    cases q4; case _ w3 w4 =>
+    have lem := classification_lemma j2; simp at lem
+    cases lem; case _ lem => cases lem
+    case _ lem =>
+    cases lem; case _ K lem =>
+    cases lem.2; case _ h1 h2 h3 =>
+    apply Judgment.empty q1
+    apply Judgment.eq q1; subst j3
+    apply beta_kind w2 h2; subst j4
+    apply beta_kind w4 h3
+  case _ =>
+    cases j2; case _ q1 q2 =>
+    cases q2; case _ q2 q3 q4 =>
+    have lem := classification_lemma j1; simp at lem
+    cases lem; case _ lem => cases lem
+    case _ lem =>
+    cases lem; case _ K lem =>
+    cases lem.2; case _ w1 w2 w3 =>
+    cases w2; case _ h1 h2 =>
+    cases w3; case _ h3 h4 =>
+    apply Judgment.empty q1
+    apply Judgment.eq q1; subst j3
+    apply beta_kind h2 q3; subst j4
+    apply beta_kind h4 q4
+  case _ =>
+    cases j1; case _ q1 q2 q3 q4 =>
+    cases q2; case _ q2 q5 q6 =>
+    cases q5; case _ w1 w2 =>
+    cases q6; case _ w3 w4 =>
+    have lem := classification_lemma j2; simp at lem
+    cases lem; case _ lem => cases lem
+    case _ lem =>
+    cases lem; case _ K lem =>
+    cases lem.2; case _ h1 h2 h3 =>
+    apply Judgment.choice q1
+    apply Judgment.eq q1; subst j3
+    apply beta_kind w2 h2; subst j4
+    apply beta_kind w4 h3
+    apply Judgment.apptc q3 j2 j3 j4
+    apply Judgment.apptc q4 j2 j3 j4
+  case _ =>
+    cases j2; case _ q1 q2 q3 q4 =>
+    cases q2; case _ q2 q5 q6 =>
+    have lem := classification_lemma j1; simp at lem
+    cases lem; case _ lem => cases lem
+    case _ lem =>
+    cases lem; case _ K lem =>
+    cases lem.2; case _ w1 w2 w3 =>
+    cases w2; case _ h1 h2 =>
+    cases w3; case _ h3 h4 =>
+    apply Judgment.choice q1
+    apply Judgment.eq q1; subst j3
+    apply beta_kind h2 q5; subst j4
+    apply beta_kind h4 q6
+    apply Judgment.apptc j1 q3 j3 j4
+    apply Judgment.apptc j1 q4 j3 j4
+case choice j1 j2 j3 j4 ih1 ih2 ih3 ih4 =>
+  cases r
+  case _ => assumption
+  case _ => assumption
+  case _ h _ => cases h
+  case _ h => cases h
+  case _ r => apply Judgment.choice j1 j2 (ih3 r) j4
+  case _ r => apply Judgment.choice j1 j2 j3 (ih4 r)
+  case _ => apply Judgment.empty j1 j2
+  case _ => apply Judgment.empty j1 j2
+  case _ h => exfalso; apply h rfl
+  case _ h => exfalso; apply h rfl
 
 theorem preservation :
   Γ ⊢ t : A ->
