SystemFD/Term/Substitution.lean
@@ -72,29 +72,34 @@ namespace Term
   unfold Term.neutral_form; rfl
 
   theorem neutral_form_app:
-  f.neutral_form = .some (h, sp) ->
-  (f `@ t).neutral_form = .some (h, sp ++ [(.term, t)]) := by
+    f.neutral_form = .some (h, sp) ->
+    (f `@ t).neutral_form = .some (h, sp ++ [(.term, t)])
+  := by
   intros h; simp_all
 
   theorem neutral_form_appt:
-  f.neutral_form = .some (h, sp) ->
-  (f `@t t).neutral_form = .some (h, sp ++ [(.type, t)])
+    f.neutral_form = .some (h, sp) ->
+    (f `@t t).neutral_form = .some (h, sp ++ [(.type, t)])
   := by intros h; simp_all
 
   theorem neutral_form_appk:
-  f.neutral_form = .some (h, sp) ->
-  (f `@k t).neutral_form = .some (h, sp ++ [(.kind, t)])
+    f.neutral_form = .some (h, sp) ->
+    (f `@k t).neutral_form = .some (h, sp ++ [(.kind, t)])
   := by intros h; simp_all
 
-  theorem unique_neutral_form : (Term.neutral_form t = .some (n, sp))
-                            -> (Term.neutral_form t = .some (n', sp')) -> (n = n' ∧ sp = sp') := by
+  theorem unique_neutral_form :
+    (Term.neutral_form t = .some (n, sp)) ->
+    (Term.neutral_form t = .some (n', sp')) ->
+    (n = n' ∧ sp = sp')
+  := by
   intros tnf tnf';
   induction t using Term.neutral_form.induct;
   any_goals (solve | simp_all)
 
   theorem neutral_form_app_rev:
-  (f `@ t).neutral_form = .some (h, sp ++ [(.term, t)] ) ->
-  f.neutral_form = .some (h, sp) := by
+    (f `@ t).neutral_form = .some (h, sp ++ [(.term, t)] ) ->
+    f.neutral_form = .some (h, sp)
+  := by
   intros h; simp_all;
   case _ n =>
   rw [Option.bind_eq_some] at h; cases h; case _ w h =>
@@ -102,8 +107,9 @@ namespace Term
   subst h2; subst h3; simp_all;
 
   theorem neutral_form_appk_rev_exists:
-  (f `@k t).neutral_form = .some (h, sp) ->
-  ∃ sp', f.neutral_form = .some (h, sp') ∧ sp = sp' ++ [(.kind , t)] := by
+    (f `@k t).neutral_form = .some (h, sp) ->
+    ∃ sp', f.neutral_form = .some (h, sp') ∧ sp = sp' ++ [(.kind , t)]
+  := by
   intros h; simp_all;
   case _ n =>
   rw [Option.bind_eq_some] at h; cases h; case _ w h =>
@@ -111,8 +117,9 @@ namespace Term
   subst h2; subst h3; simp_all;
 
   theorem neutral_form_appt_rev:
-  (f `@t t).neutral_form = .some (h, sp ++ [(.type, t)] ) ->
-  f.neutral_form = .some (h, sp) := by
+    (f `@t t).neutral_form = .some (h, sp ++ [(.type, t)] ) ->
+    f.neutral_form = .some (h, sp)
+  := by
   intros h; simp_all;
   case _ n =>
   rw [Option.bind_eq_some] at h; cases h; case _ w h =>
